working on main dijstra function

dafny/dijkstra.dfy
@@ -33,9 +33,6 @@ class Graph{
    this.vertices.Length == size  &&
    forall n :: 0 <= n < this.vertices.Length ==> this.vertices[n] != null &&
    forall m :: 0 <= m < this.edgeweights.Length ==> (this.edgeweights[m] != null && this.edgeweights[m].Length == size)
-   /* forall h :: 0 <= h < vertices.Length ==> (vertices[h].wfs != 900000 && vertices[h].pred != 900000) &&
-   forall x :: 0 <= x < edgeweights.Length ==> edgeweights[x].Length == edgeweights.Length  &&
-   forall s, d :: 0  <= s < edgeweights.Length && 0 <= d < edgeweights[s].Length ==>  edgeweights[s][d] > 0 */
   }
 
   predicate edges()
@@ -80,6 +77,18 @@ class MinQueue{
 	  Repre := Repre + {vertex};
 	}
 
+	method getSize() returns (size:int)
+	{
+	size := |Repre|;
+	return size;
+	}
+
+	predicate isEmpty()
+	reads this, this.Repre
+	{
+	Repre == {}
+	}
+
 	method removeMin() returns (v: Vertex) // remove the smallest integer from the queue and return it
 	modifies this;                              // since we represent each vertex in the Graph object as its entry in "vertices"
 	requires Repre != {};                       // we need only know which entry has the minimum wfs in the queue
@@ -111,9 +120,8 @@ class MinQueue{
 	 modifies set m | 0 <= m < G.vertices.Length  :: G.vertices[m]
 	 ensures G.isValid() && G.verticesValid() && G.hasVertex(s)
 	 ensures G.vertices != null 
-	 ensures G.vertices[s].wfs == 0 //&& G.vertices[s].wfs == 900000
+	 ensures G.vertices[s].wfs == 0 && G.vertices[s].pred == 900000
    {
-     assert G.vertices != null;
      var x := 0 ;
 	 while x < G.vertices.Length
 	 modifies set m | 0 <= m < G.vertices.Length :: G.vertices[m]
@@ -126,15 +134,56 @@ class MinQueue{
 	 G.vertices[x].pred := 900000;
      x := x + 1 ;
 	 }
-	 //assert G.vertices[s].pred == 900000;
 	 G.vertices[s].wfs := 0;
+	 G.vertices[s].pred := 900000;
    }
 
-   method relax(G: Graph, u: int, v: int, w: int)
-	reads G, G.edgeweights
-	reads set m |  0 <= m < G.edgeweights.Length :: G.edgeweights[m]
+  method relax(G: Graph, u: int, v: int)
 	requires G != null && G.isValid() && G.hasVertex(u) && G.hasVertex(v) && G.edges()
 	modifies G, G.edgeweights
-	modifies set m |  0 <= m < G.edgeweights.Length :: G.edgeweights[m]
-   {}
-   } 
+	//modifies set m |  0 <= m < G.edgeweights.Length :: G.edgeweights[m]
+	modifies set n | 0 <= n < G.vertices.Length :: G.vertices[n]
+   {
+   if (G.vertices[v].wfs > G.vertices[u].wfs + G.edgeweights[u][v])
+	{
+		G.vertices[v].wfs := G.vertices[u].wfs + G.edgeweights[u][v];
+		G.vertices[v].pred := u;
+	}
+   }
+ 
+   method sssp(G:Graph, source: int)
+   requires G != null 
+   requires G.isValid() && G.hasVertex(source) && G.verticesValid()
+   requires G.edges()
+   modifies G, G.vertices, G.edgeweights
+   modifies set m | 0 <= m < G.vertices.Length :: G.vertices[m]
+   {
+
+   InitializeSS(G,source);
+   var finishedVertices : set<Vertex> := {};
+   var Q := new MinQueue.Init();
+   var u := new Vertex.Init();
+   var i := 0;
+   
+   
+   while i < G.vertices.Length
+	invariant G.isValid()
+	invariant G.hasVertex(source) && G.verticesValid()
+	{
+		Q.addV(G.vertices[i]);
+		i := i + 1;
+	}
+
+   while !Q.isEmpty()
+	invariant G.isValid()
+	invariant G.hasVertex(source) && G.verticesValid()
+	modifies  G, G.vertices, G.edgeweights
+	modifies Q
+	modifies set m | 0 <= m < G.vertices.Length :: G.vertices[m]
+	{
+		u:= Q.removeMin();
+	}
+
+   }
+   }
+    
